Affine/Normalize.lean
@@ -38,70 +38,6 @@ def small_step (e : Lambda) : Lambda :=
       (add_le_add (e₁.small_step_count x) (e₂.small_step_count x))
       (e₃.small_step_count x)
 
-theorem small_step_count_β_eq_zero {e : Lambda} (h : e.count_β = 0) : e.small_step.count_β = 0 := by
-  match e with
-  | .var _ => simp only [count_β]
-  | .abs _ e =>
-    simp only [count_β] at h
-    simp only [count_β, small_step_count_β_eq_zero h]
-  | .app (.var _) e₂ =>
-    simp only [count_β] at h
-    simp only [count_β, small_step_count_β_eq_zero h]
-  | .app (.abs x e₁) e₂ =>
-    simp_rw [count_β, add_assoc, add_comm 1, Nat.add_one_ne_zero] at h
-  | .app (.app e₁ e₂) e₃ =>
-    simp only [count_β, Nat.add_eq_zero_iff] at h
-    have ⟨⟨he₁, he₂⟩, he₃⟩ := h
-    simp only [count_β, he₁, he₂, he₃, small_step_count_β_eq_zero]
-
-theorem small_step_count_β_lt {e : Lambda} (h₁ : e.count_β ≠ 0) (h₂ : e.is_affine) :
-    e.small_step.count_β < e.count_β := by
-  match e with
-  | .var x => simp only [count_β, ne_eq, not_true_eq_false] at h₁
-  | .abs _ e
-  | .app (.var _) e₂ =>
-    simp only [count_β] at h₁
-    simp [is_affine, decide_eq_true_eq] at h₂
-    simp only [count_β, small_step_count_β_lt h₁ h₂.left]
-  | .app (.abs x e₁) e₂ =>
-    simp only [count_β, is_affine, decide_eq_true_eq] at h₁ h₂
-    have ⟨⟨he₁, _⟩, he₂, _⟩ := h₂
-    simp only [count_β, small_step]
-  | .app (.app e₁ e₂) e₃ =>
-    simp only [count_β, is_affine, decide_eq_true_eq] at h₁ h₂
-    have ⟨⟨ha₁, ha₂, _⟩, ha₃, _⟩ := h₂
-    simp only [count_β, small_step]
-
-    /-
-      lots of code to just show this:
-      h : count_β e₁ + count_β e₂ + count_β e₃ ≠ 0
-      ⊢ e₁.small_step.count_β + e₂.small_step.count_β + e₂.small_step.count_β <
-          e₁.count_β + e₂.count_β + e₃.count_β
-    -/
-    by_cases he₁ : e₁.count_β = 0
-    · simp only [he₁, small_step_count_β_eq_zero, zero_add]
-      by_cases he₂ : e₂.count_β = 0
-      · simp only [he₁, he₂, zero_add] at h₁
-        simp only [he₂, small_step_count_β_eq_zero, zero_add, small_step_count_β_lt h₁ ha₃]
-      · by_cases he₃ : e₃.count_β = 0
-        · simp only [he₁, he₃, add_zero, zero_add] at h₁
-          simp only [he₃, small_step_count_β_eq_zero, small_step_count_β_lt he₂ ha₂,
-            zero_add, add_zero]
-        · exact add_lt_add (small_step_count_β_lt he₂ ha₂) (small_step_count_β_lt he₃ ha₃)
-    · by_cases he₂ : e₂.count_β = 0
-      · by_cases he₃ : e₃.count_β = 0
-        · simp only [he₂, he₃, add_zero] at h₁
-          simp only [he₂, he₃, small_step_count_β_eq_zero, add_zero, small_step_count_β_lt he₁ ha₁]
-        · simp only [he₂, small_step_count_β_eq_zero, add_zero]
-          exact add_lt_add (small_step_count_β_lt he₁ ha₁) (small_step_count_β_lt he₃ ha₃)
-      · by_cases he₃ : e₃.count_β = 0
-        · simp only [he₃, small_step_count_β_eq_zero, add_zero,
-          add_lt_add (small_step_count_β_lt he₁ ha₁) (small_step_count_β_lt he₂ ha₂)]
-        · refine' add_lt_add (add_lt_add _ _) _
-          · exact small_step_count_β_lt he₁ ha₁
-          · exact small_step_count_β_lt he₂ ha₂
-          · exact small_step_count_β_lt he₃ ha₃
-
 @[simp] theorem small_step_is_affine {e : Lambda} (h : e.is_affine) : e.small_step.is_affine := by
   match e with
   | .var x => simp only [small_step, h]
@@ -143,6 +79,63 @@ theorem small_step_count_β_lt {e : Lambda} (h₁ : e.count_β ≠ 0) (h₂ : e.
         (Finset.union_subset_union e₁.small_step_free e₂.small_step_free)
         e₃.small_step_free
 
+theorem small_step_size_le {e : Lambda} (he : e.is_affine) :
+    e.small_step.size ≤ e.size := by
+  match e with
+  | .var x => rfl
+  | .abs x e =>
+    simp only [is_affine_of_abs] at he
+    exact add_le_add_left (e.small_step_size_le he.1) _
+  | .app (.var x) e =>
+    simp only [is_affine_of_app, is_affine_of_var, true_and, free] at he
+    simp only [size, zero_add, e.small_step_size_le he.1]
+  | .app (.app e₁ e₂) e₃ =>
+    simp only [is_affine_of_app, true_and, free] at he
+    have ⟨⟨he₁, he₂, _⟩, he₃, _⟩ := he
+    simp only [size]
+    refine' add_le_add _ (e₃.small_step_size_le he₃)
+    refine' add_le_add (e₁.small_step_size_le he₁) (e₂.small_step_size_le he₂)
+  | .app (.abs x e₁) e₂ =>
+    simp only [is_affine_of_app, is_affine_of_abs, free] at he
+    simp only [size, small_step]
+    apply le_of_lt
+    exact substₑ_size_lt he.1.1
+
+theorem small_step_size_lt {e : Lambda} (he : e.is_affine) (hβ : e.count_β ≠ 0) :
+    e.small_step.size < e.size := by
+  match e with
+  | .var x => simp only [count_β] at hβ; contradiction
+  | .abs x e =>
+    simp only [count_β, is_affine_of_abs] at he hβ
+    simp only [size, small_step, add_lt_add_left (small_step_size_lt he.1 hβ) 1]
+  | .app (.var x) e₂ =>
+    simp only [count_β_of_app_var, is_affine_of_app, is_affine_of_var, true_and] at he hβ
+    simp only [size, zero_add, small_step_size_lt he.1 hβ]
+  | .app (.app e₁ e₂) e₃ =>
+    simp only [count_β_of_app_app, is_affine_of_app] at he hβ
+    have ⟨⟨he₁, he₂, _⟩, he₃, _⟩ := he
+    simp only [size]
+    have hdisj := add_add_neq_zero hβ
+    refine' Or.elim hdisj (fun hβ₁ => _) (fun hβ₂₃ => Or.elim hβ₂₃ (fun hβ₂ => _) (fun hβ₃ => _))
+    · apply add_lt_add_of_lt_of_le
+      apply add_lt_add_of_lt_of_le
+      exact small_step_size_lt he₁ hβ₁
+      exact small_step_size_le he₂
+      exact small_step_size_le he₃
+    · apply add_lt_add_of_lt_of_le
+      apply add_lt_add_of_le_of_lt
+      exact small_step_size_le he₁
+      exact small_step_size_lt he₂ hβ₂
+      exact small_step_size_le he₃
+    · apply add_lt_add_of_le_of_lt
+      apply add_le_add
+      exact small_step_size_le he₁
+      exact small_step_size_le he₂
+      exact small_step_size_lt he₃ hβ₃
+  | .app (.abs x e₁) e₂ =>
+    simp only [count_β_of_app_abs, is_affine_of_app, is_affine_of_abs] at he hβ
+    simp only [size, small_step, substₑ_size_lt he.1.1]
+
 end Lambda
 
 namespace Affine
@@ -155,17 +148,22 @@ def small_step_impl (e : Affine vs) : (vs' : Finset ℕ) × (Affine vs') :=
 def small_step_free (e : Affine vs) : Finset ℕ := e.small_step_impl.1
 def small_step (e : Affine vs) : Affine e.small_step_free := e.small_step_impl.2
 
-theorem small_step_count_β_lt {e : Affine vs} (hβ : e.count_β ≠ 0) :
-    e.small_step.count_β < e.count_β := by
-  simp only [small_step, small_step_impl, ← to_lambda_count_β_eq, Lambda.of_lambda_to_lambda]
-  apply Lambda.small_step_count_β_lt (e.to_lambda_count_β_eq ▸ hβ) e.to_lambda_is_affine
+theorem to_lambda_small_step {e : Affine vs} :
+    e.to_lambda.small_step = e.small_step.to_lambda := by
+  sorry
+
+theorem small_step_size_lt {e : Affine vs} (hβ : e.count_β ≠ 0) :
+    e.small_step.size < e.size := by
+  rw [← to_lambda_count_β_eq] at hβ
+  rw [← e.small_step.to_lambda_size_eq, ← e.to_lambda_size_eq, ← e.to_lambda_small_step]
+  exact Lambda.small_step_size_lt e.to_lambda_is_affine hβ
 
 def normalize (e : Affine vs) : (vs' : Finset ℕ) × (Affine vs') :=
   if hβ : e.count_β = 0 then
     ⟨vs, e⟩
   else
-    have := small_step_count_β_lt hβ
+    have := small_step_size_lt hβ
     normalize e.small_step
-termination_by e.count_β
+termination_by e.size
 
 end Affine
